***2-3 Correctness of Horner's rule***<br>
The following code fragment impelements Horner's rule for evaluating a polynomial

*P*(*x*) = Σ<sup>*n*</sup><sub>*k*=0</sub> = a<sub>k</sub> x<sup>k</sup> = *a*<sub>0</sub> + *x*(*a*<sub>1</sub> + *x*(*a*<sub>2</sub> + ... + *x(a*<sub>*n*-1</sub> + *xa<sub>n</sub>*) ... )),

given the coefficients *a*<sub>0</sub>, *a*<sub>1</sub>, ... ,*a*<sub>n</sub> and a value for *x*:
```
y = 0
for i = n downto 0
    y = a_i + x*y
```
***a.*** In terms of Θ-notation, what is the running time of this code fragment for Horner's rule?
* Θ(n)

***b.*** Write pseudocode to implement the naive polynomial evaluation that computes each term from scratch. What is the running time of this algorithm? How does it compare to Horner's rule?
```
# Treating power as non-primitive operation

y = 0
for j = 0 to n
    # first compute x term by multiplication
    hold = 1
    for i = 1 to j
        hold = hold * x

    y = y + a_j * hold
```
* Running time is Θ(n<sup>2</sup>), which is worse than using Horner's rule

***c.*** Consider the following loop invariant:

At the start of each iternation of the **for** loop of lines 2–3,<br>
y = Σ<sub>k=0</sub><sup>n-(i+1)</sup> [a<sub>k+i+1</sub>x<sup>k</sup>]

Interpret a summation with no terms as equalling 0. Following the structure of the loop invariant proof presented in this chapter, use this loop invariant to show that, at termination, y = Σ<sup>n</sup><sub>k=0</sub> a<sub>k</sub>x<sup>k</sup>
* **Initialisation:** Initially, i = n such that k ranges from 0 to n-(n+1) = -1. Hence, y = 0.
* **Maintenence:** Every iteration of the loop, we get:<br>
y = a<sub>i</sub> + x · Σ<sub>k=0</sub><sup>n-(i+1)</sup> [a<sub>k+i+1</sub>x<sup>k</sup>] = a<sub>i</sub> + Σ<sub>k=0</sub><sup>n-i-1</sup> [a<sub>k+i+1</sub>x<sup>k+1</sup>] = a<sub>i</sub> + Σ<sup>n-i</sup><sub>k=1</sub> [a<sub>k+i</sub>x<sup>k</sup>] = Σ<sup>n-i</sup><sub>k=0</sub> [a<sub>k+i+1</sub>x<sup>k</sup>]
* **Termination:** The loop terminates when i = -1. Substituting this results in:<br>
y = Σ<sub>k=0</sub><sup>n-(-1+1)</sup> [a<sub>k-1+1</sub>x<sup>k</sup>] = Σ<sup>n</sup><sub>k=0</sub> a<sub>k</sub>x<sup>k</sup>

***d.*** Conclude by arguing that the given code fragment correctly evaluates a polynomial characterised by the coefficients *a*<sub>0</sub>, *a*<sub>1</sub>, ..., *a*<sub>n</sub>.
* The loop invariant shows that the evaluated sum would result in a polynomial with the given coefficients